DinD: Use subset types to capture well-formedness in the translator
It was surprisingly tricky to get this to work:

- Switching to subset types caused verification errors on all paths creating
  values in those types. (https://github.com/dafny-lang/dafny/issues/2107)
- Adding `{:fuel 2}` on `All_Expr` fixed those errors, but created new ones in
  module `Rec` (https://github.com/dafny-lang/dafny/issues/2109) and in the
  proof of equivalence between `Rec` and `NonRec`.
- Copying the body of `All_Expr` into a postcondition instead caused an infinite
  loop (in the verification of EliminateNegatedBinops_Expr_direct?)

The trick that worked best in the end was eliminating the mutual recursion by
inlining AllExpr_Children into AllExpr.  Doing so also revealed a missing
`decreases` clause, https://github.com/dafny-lang/dafny/issues/2110

Source/DafnyCompilers/CSharpDafnyASTInterop.dfy
@@ -3,10 +3,17 @@ include "CSharpDafnyASTModel.dfy"
 module {:extern "CSharpDafnyASTInterop"} CSharpDafnyASTInterop {
   import CSharpDafnyASTModel
 
+  function {:axiom} TypeHeight(t: CSharpDafnyASTModel.Type) : nat
+
+  function {:axiom} ASTHeight(c: object) : nat
+    requires || c is CSharpDafnyASTModel.Expression
+             || c is CSharpDafnyASTModel.Statement
+
   class {:extern} TypeUtils {
     constructor {:extern} () requires false // Prevent instantiation
 
     static function method {:extern} NormalizeExpand(ty: CSharpDafnyASTModel.Type)
-      : CSharpDafnyASTModel.Type
+      : (ty': CSharpDafnyASTModel.Type)
+      ensures TypeHeight(ty') <= TypeHeight(ty)
   }
 }
